Proof/Theorem2.lean
@@ -1,0 +1,12 @@
+import Proof.Semantics
+import Proof.Analysis
+import Proof.CorrectnessRelation
+
+namespace Proof
+
+theorem partially_init_obj_on_stack {Γ : GTable} {G : GlobName} {uᵢ u₁ u₂ : GVal}
+    {S : Stack} (hG : Γ G = (GEntry.mk u₁ u₂)) (hsel : uᵢ = u₁ ∨ uᵢ = u₂)
+    (hnone : uᵢ = none) : inGlobals G S :=
+  sorry
+
+end Proof
